list_of_vlsms.v
@@ -166,6 +166,24 @@ destruct Ss as [| Sh St]; unfold composed_label; unfold composed_state; simpl
     * exact (composed_valid _ St lt (st, None)).
 Defined.
 
+Lemma composed_valid_decidable
+  {message}
+  (Ss : list (VLSM message))
+  : forall l som, {composed_valid Ss l som} + {~composed_valid Ss l som}.
+Proof.
+  induction Ss as [| Sh St]; unfold composed_label; unfold composed_state; simpl; intros l [s om].
+  - inversion l.
+  - destruct s as [sh st]. destruct om as [[m Hm]|].
+    + destruct l as [lh | lt].
+      * destruct (@proto_message_decidable _ Sh m) as [Hh | _]; try (right; intro; contradiction).
+        apply valid_decidable.
+      * destruct (composed_proto_message_decidable St m) as [Ht | _]; try (right; intro; contradiction).
+        apply IHSt.
+    + destruct l as [lh | lt].
+      * apply valid_decidable.
+      * apply IHSt.
+Qed.
+
 Definition composed_valid_constrained
   {message}
   (Ss : list (VLSM message))
@@ -174,6 +192,25 @@ Definition composed_valid_constrained
   (som : composed_state Ss * option (composed_proto_message Ss) )
   :=
   composed_valid Ss l som /\ constraint l som.
+
+
+Lemma composed_valid_constrained_decidable
+  {message}
+  (Ss : list (VLSM message))
+  {constraint : composed_label Ss -> composed_state Ss * option (composed_proto_message Ss) -> Prop}
+  (constraint_decidable : forall (l : composed_label Ss) (som : composed_state Ss * option (composed_proto_message Ss)), {constraint l som} + {~constraint l som})
+  (l : composed_label Ss)
+  (som : composed_state Ss * option (composed_proto_message Ss) )
+  : {composed_valid_constrained Ss constraint l som} + {~composed_valid_constrained Ss constraint l som}.
+Proof.
+  unfold composed_valid_constrained.
+  destruct (constraint_decidable l som) as [Hc | Hnc].
+  - destruct (composed_valid_decidable Ss l som) as [Hv | Hnv].
+    + left. split; try assumption.
+    + right. intros [Hv _]. contradiction.
+  - right. intros [_ Hc]. contradiction.
+Qed.
+
 
 Definition composed_vlsm
   {message}
@@ -192,6 +229,7 @@ Definition composed_vlsm
   ; label_inhabited := composed_label_inhabited Ss Ssnn
   ; transition := composed_transition Ss
   ; valid := composed_valid Ss
+  ; valid_decidable := composed_valid_decidable Ss
   |}.
 
 Definition composed_vlsm_constrained
@@ -199,6 +237,7 @@ Definition composed_vlsm_constrained
   (Ss : list (VLSM message))
   (Ssnn : Ss <> [])
   (constraint : composed_label Ss -> composed_state Ss * option (composed_proto_message Ss) -> Prop)
+  (constraint_decidable : forall (l : composed_label Ss) (som : composed_state Ss * option (composed_proto_message Ss)), {constraint l som} + {~constraint l som})
   : VLSM message
   :=
   {| state := composed_state Ss
@@ -212,4 +251,5 @@ Definition composed_vlsm_constrained
   ; label_inhabited := composed_label_inhabited Ss Ssnn
   ; transition := composed_transition Ss
   ; valid := composed_valid_constrained Ss constraint
+  ; valid_decidable := composed_valid_constrained_decidable Ss constraint_decidable
   |}.
