two_vlsms.v
@@ -161,6 +161,25 @@ destruct som as [[s1 s2] [[m Hm]|]].
   + exact (valid l2 (s2, None)).
 Defined.
 
+Lemma composed2_valid_decidable
+  {message}
+  (S1 : VLSM message)
+  (S2 : VLSM message)
+  (l : (@label message S1) + (@label message S2))
+  (som : ((@state message S1) * (@state message S2)) * option (composed2_proto_message S1 S2))
+  : {composed2_valid S1 S2 l som} + {~composed2_valid S1 S2 l som}.
+Proof.
+  destruct som as [[s1 s2] [[m Hm]|]].
+  - destruct l as [l1 | l2]; simpl.
+    + destruct (@proto_message_decidable _ S1 m) as [H1 | _].
+      * apply valid_decidable.
+      * right. intro. assumption.
+    + destruct (@proto_message_decidable _ S2 m) as [H2 | _].
+      * apply valid_decidable.
+      * right. intro. assumption.
+  - destruct l as [l1 | l2]; simpl; apply valid_decidable.
+Qed.
+
 Definition composed2_valid_constrained
   {message}
   (S1 : VLSM message)
@@ -170,6 +189,24 @@ Definition composed2_valid_constrained
   (som : ((@state message S1) * (@state message S2)) * option (composed2_proto_message S1 S2))
   :=
   composed2_valid S1 S2 l som /\ constraint l som.
+
+Lemma composed2_valid_constraint_decidable
+  {message}
+  (S1 : VLSM message)
+  (S2 : VLSM message)
+  {constraint : (@label message S1) + (@label message S2) -> ((@state message S1) * (@state message S2)) * option (composed2_proto_message S1 S2) -> Prop}
+  (constraint_decidable : forall (l : (@label message S1) + (@label message S2)) (som : ((@state message S1) * (@state message S2)) * option (composed2_proto_message S1 S2)), {constraint l som} + {~constraint l som})
+  (l : (@label message S1) + (@label message S2))
+  (som : ((@state message S1) * (@state message S2)) * option (composed2_proto_message S1 S2))
+  : {composed2_valid_constrained S1 S2 constraint l som} + {~composed2_valid_constrained S1 S2 constraint l som}.
+Proof.
+  unfold composed2_valid_constrained.
+  destruct (constraint_decidable l som) as [Hc | Hnc].
+  - destruct (composed2_valid_decidable S1 S2 l som) as [Hv | Hnv].
+    + left. split; try assumption.
+    + right. intros [Hv _]. contradiction.
+  - right. intros [_ Hc]. contradiction.
+Qed.
 
 Definition compose2_vlsm
   {message}
@@ -188,6 +225,7 @@ Definition compose2_vlsm
   ; label_inhabited := composed2_label_inhabited S1 S2
   ; transition := composed2_transition S1 S2
   ; valid := composed2_valid S1 S2
+  ; valid_decidable := composed2_valid_decidable S1 S2
   |}.
 
 Definition compose2_vlsm_constrained
@@ -195,6 +233,7 @@ Definition compose2_vlsm_constrained
   (S1 : VLSM message)
   (S2 : VLSM message)
   (constraint : (@label message S1) + (@label message S2) -> (@state message S1 * @state message S2) * option (composed2_proto_message S1 S2) -> Prop)
+  (constraint_decidable : forall (l : (@label message S1) + (@label message S2)) (som : ((@state message S1) * (@state message S2)) * option (composed2_proto_message S1 S2)), {constraint l som} + {~constraint l som})
   : VLSM message
   :=
   {| state := (@state message S1) * (@state message S2)
@@ -208,4 +247,5 @@ Definition compose2_vlsm_constrained
   ; label_inhabited := composed2_label_inhabited S1 S2
   ; transition := composed2_transition S1 S2
   ; valid := composed2_valid_constrained S1 S2 constraint
+  ; valid_decidable := composed2_valid_constraint_decidable S1 S2 constraint_decidable
   |}.
